---
title: "Dynamic Asset Pricing Models"
subtitle: "Asset Pricing Theory"
author: "Juan F. Imbet"
institute: "Paris Dauphine University-PSL"
format:
  revealjs:
    theme: white
    css: ../../../assets/styles.css
    slide-number: true
    chalkboard: true
    preview-links: auto
    footer: "Asset Pricing Theory - Dynamic Asset Pricing Models"
execute:
  enabled: false
---

## Dynamic Asset Pricing Models {.center}

**Hamilton-Jacobi-Bellman Equations and Term Structure Models**

### Basic Setup and Assumptions

**Assumptions:**

- **Time horizon:** Infinite horizon $t \in [0, \infty)$
- **Investment opportunity set:** Single risky asset with return dynamics
- **Investor preferences:** Time-separable utility with constant relative risk aversion
- **Markets:** Frictionless, continuous trading
- **Information:** Full information about state variables

**State variables:**

- Wealth: $W_t$ (investor's financial wealth)
- Time: $t$ (for time-varying preferences/parameters)

**Controls:**

- Consumption: $C_t \geq 0$
- Portfolio allocation: $\omega_t$ (fraction in risky asset)

---

## The HJB Equation in Continuous-Time Optimization

- The HJB equation arises from the dynamic programming principle. The solution to a continuous-time optimization problem can be characterized by a partial differential equation (PDE) known as the HJB equation.

**General Case**:

- Assume a general dynamic optimization problem with state variable $X_t$ and control variable $u_t$.

$$
dX_t = \mu(X_t, u_t) dt + \sigma(X_t, u_t) dW_t
$$

- Standard Discounted Utility:

$$
\max_{u_t} E_t \left[ \int_t^\infty e^{-\rho (s-t)} U(X_s, u_s) ds \right]
$$

**HJB Equation:**

$$
\rho V(X_t, t) = \max_{u_t} \left\{ U(X_t, u_t) + \frac{\partial V}{\partial t} + \frac{\partial V}{\partial X} \mu(X_t, u_t) + \frac{1}{2} \frac{\partial^2 V}{\partial X^2} \sigma^2(X_t, u_t) \right\}
$$

where $\mu(X_t, u_t) = \text{drift of } X_t$, $\sigma^2(X_t, u_t) = \text{variance of } X_t$

---

## The Hamilton-Jacobi-Bellman Equation in Dynamic Portfolio Choice

- A representative investor chooses how much to consume and how to allocate wealth between a risky asset and a risk-free asset to maximize expected utility over an infinite horizon. $\omega_t$ is the fraction of wealth invested in the risky asset.

**Value function definition:**

$$
V(W, t) = \max_{C_s, \omega_s} E_t\left[ \int_t^\infty e^{-\rho(s-t)} U(C_s) ds \right]
$$

**Dynamic programming principle:**

$$
V(W, t) = \max_{C, \omega} \left\{ U(C) + E_t\left[ V(W_{t+dt}, t+dt) \right] \right\}
$$

**Taylor expansion:**

$$
V(W + dW, t + dt) \approx V(W,t) + V_t dt + V_W dW + \frac{1}{2} V_{WW} (dW)^2
$$

---

## Wealth Dynamics (continued)

**HJB equation derivation:**

$$
\rho V(W,t) = \max_{C,\omega} \left\{ U(C) + \frac{\partial V}{\partial t} + \frac{\partial V}{\partial W} \mu_W + \frac{1}{2} \frac{\partial^2 V}{\partial W^2} \sigma_W^2 \right\}
$$

where:

- $\mu_W = \omega W \mu + (1-\omega) W r - C = \omega W (\mu - r) + W r - C$ (wealth drift)
- $\sigma_W^2 = W^2 \omega^2 \sigma^2$ (wealth variance)

**Final HJB equation:**

$$
\rho V(W,t) = \max_{C,\omega} \left\{ U(C) + \frac{\partial V}{\partial t} + \frac{\partial V}{\partial W} [r W + \omega W (\mu - r) - C] + \frac{1}{2} \frac{\partial^2 V}{\partial W^2} W^2 \omega^2 \sigma^2 \right\}
$$

---

## Power Utility Solution

### Assumptions for Power Utility

**Utility function:**

$$
U(C) = \frac{C^{1-\gamma}}{1-\gamma}, \quad \gamma > 0, \gamma \neq 1
$$
**Key properties:**

- Constant relative risk aversion: $RRA = -\frac{U''(C) C}{U'(C)} = \gamma$
- Elasticity of intertemporal substitution: $EIS = \frac{1}{\gamma}$
- Solving a HJB required a guess for the value function. How it depends on wealth and time.
- A common assumption that simplifies the problem is to assume that the value function is separable in wealth and time.

**Guess for value function:**

$$
V(W,t) = \frac{1}{1-\gamma} W^{1-\gamma} v(t)
$$

**Motivation:** Homothetic preferences (scaling wealth scales utility proportionally) allow separation of wealth and time effects.

---

## Step-by-Step HJB Solution

**Substitute guess into HJB:**

$$
\rho \cdot \frac{1}{1-\gamma} W^{1-\gamma} v(t) = \max_{C,\omega} \left\{ \frac{C^{1-\gamma}}{1-\gamma} + \frac{\partial V}{\partial t} + V_W [r W + \omega W (\mu - r) - C] + \frac{1}{2} V_{WW} W^2 \omega^2 \sigma^2 \right\}
$$

**Compute partial derivatives:**

$$
\frac{\partial V}{\partial t} = \frac{1}{1-\gamma} W^{1-\gamma} v'(t)
$$
$$
\frac{\partial V}{\partial W} = W^{-\gamma} v(t)
$$
$$
\frac{\partial^2 V}{\partial W^2} = -\gamma W^{-\gamma-1} v(t)
$$

**Substitute derivatives:**

$$
\rho v(t) W^{1-\gamma} = \max_{C,\omega} \left\{ \frac{C^{1-\gamma}}{1-\gamma} + W^{1-\gamma} v'(t) + W^{-\gamma} v(t) [r W + \omega W (\mu - r) - C] + \frac{1}{2} (-\gamma W^{-\gamma-1} v(t)) W^2 \omega^2 \sigma^2 \right\}
$$

**Divide both sides by $W^{1-\gamma}$:**

$$
\rho v(t) = \max_{C,\omega} \left\{ \frac{C^{1-\gamma}}{1-\gamma} W^{-\gamma} + v'(t) + v(t) [r + \omega (\mu - r) - C W^{-1}] - \frac{1}{2} \gamma v(t) \omega^2 \sigma^2 \right\}
$$

---

## Continued HJB Solution

**First-order condition for consumption:**

$$
\frac{\partial}{\partial C} \left[ \frac{C^{1-\gamma}}{1-\gamma} W^{-\gamma} - v(t) C W^{-1} \right] = 0
$$
$$
C^{-\gamma} W^{-\gamma} - v(t) W^{-1} = 0
$$
$$
C^{-\gamma} = v(t) W^{-1}
$$
C^* = [v(t) W^{-1}]^{-1/\gamma} = W \cdot v(t)^{1/\gamma}
$$

**First-order condition for portfolio:**

$$
\frac{\partial}{\partial \omega} [v(t) \omega (\mu - r) - \frac{1}{2} \gamma v(t) \omega^2 \sigma^2] = 0
$$
$$
v(t) (\mu - r) - \gamma v(t) \omega \sigma^2 = 0
$$
$$
\omega^* = \frac{\mu - r}{\gamma \sigma^2}
$$

**Substitute optimal controls back into HJB:**

$$
\rho v(t) = \frac{[W \cdot v(t)^{1/\gamma}]^{1-\gamma}}{1-\gamma} W^{-\gamma} + v'(t) + v(t) \left[ r + \frac{\mu - r}{\gamma \sigma^2} (\mu - r) - v(t)^{1/\gamma} \right] - \frac{1}{2} \gamma v(t) \left( \frac{\mu - r}{\gamma \sigma^2} \right)^2 \sigma^2
$$

---

## Continued HJB Solution

**Simplify step by step:**

$$
\begin{align*}
\rho v(t) &= \frac{v(t)}{1-\gamma} + v'(t) + r v(t) + \frac{(\mu - r)^2}{\gamma \sigma^2} v(t) - v(t)^{1 + 1/\gamma} - \frac{(\mu - r)^2}{2 \gamma \sigma^2} v(t) \\
\rho v(t) &= v'(t) + \frac{v(t)}{1-\gamma} + r v(t) + \frac{(\mu - r)^2}{2 \gamma \sigma^2} v(t) - v(t)^{1 + 1/\gamma} \\
\rho v(t) &= v'(t) + v(t) \left[ \frac{1}{1-\gamma} + r + \frac{(\mu - r)^2}{2 \gamma \sigma^2} \right] - v(t)^{1 + 1/\gamma} \\
v'(t) + \Big[ \tfrac{1}{1-\gamma} + r + \tfrac{(\mu - r)^2}{2 \gamma \sigma^2} - \rho \Big] v(t) &= v(t)^{1 + 1/\gamma}\\
v'(t) &= \Big[ \rho - \tfrac{1}{1-\gamma} - r - \tfrac{(\mu - r)^2}{2 \gamma \sigma^2} \Big] v(t) + v(t)^{1 + 1/\gamma}
\end{align*}
$$

- This is a nonlinear ODE (Bernoulli type): 
$$
v'(t) = a\,v(t) + b\,v(t)^{1+1/\gamma}
$$

---

## Bernoulli reduction and solution (step by step)

Let $a,b\in\mathbb{R}$ and $\gamma>0$. Consider
$$
v'(t)= a\,v(t)+b\,v(t)^{1+1/\gamma}.
$$

**1) Substitution.** Set
$$
u(t)=v(t)^{-1/\gamma}\quad\Longrightarrow\quad u'(t)
= -\frac{1}{\gamma}\,v(t)^{-1/\gamma-1}\,v'(t).
$$

**2) Express $u'$ using the ODE.** From the ODE,
$$
v'(t)=a\,v(t)+b\,v(t)^{1+1/\gamma}.
$$
Multiply both sides by $-\dfrac{1}{\gamma}v(t)^{-1/\gamma-1}$:
$$
-\frac{1}{\gamma}v^{-1/\gamma-1}v'
= -\frac{a}{\gamma}v^{-1/\gamma}-\frac{b}{\gamma}.
$$
The left-hand side is exactly $u'(t)$, and $v^{-1/\gamma}=u$, hence
$$
u'(t)+\frac{a}{\gamma}u(t)=-\frac{b}{\gamma}.
$$

- This is a linear ODE in $u$. 

---

## Linear ODEs

Consider the general linear ODE

$$
u'(t) = a u(t) + b,
$$
where $a,b \in \mathbb{R}$.

The solution is given by
$$
u(t) = -\frac{b}{a} + C e^{a t},\qquad C \in \mathbb{R},
$$

Check by differentiation:
$$
u'(t) = C a e^{a t} = a \left( -\frac{b}{a} + C e^{a t} \right) + b = a u(t) + b.
$$

---

## Continued Bernoulli reduction and solution

- Back to our setup, we have

$$
u'(t) = - \frac{a}{\gamma} u(t)  -\frac{b}{\gamma}.
$$

- The solution is
$$
u(t) = -\frac{-b/\gamma}{-a/\gamma} + C e^{-\frac{a}{\gamma} t} = -\frac{b}{a} + C e^{-\frac{a}{\gamma} t},\qquad C \in \mathbb{R}.
$$

Compute $C$ using initial condition $u(0) = v(0)^{-1/\gamma}$:

$$
u(0) = -\frac{b}{a} + C = v(0)^{-1/\gamma} \implies C = v(0)^{-1/\gamma} + \frac{b}{a}.
$$

- Hence

$$
u(t) = -\frac{b}{a} + \left( v(0)^{-1/\gamma} + \frac{b}{a} \right) e^{-\frac{a}{\gamma} t}.
$$

$$
v(t) = \left( -\frac{b}{a} + \left( v(0)^{-1/\gamma} + \frac{b}{a} \right) e^{-\frac{a}{\gamma} t} \right)^{-\gamma}.
$$

---

## Original parameters

Recall that

$$
\begin{align*}
a &= \Big[ \rho - \tfrac{1}{1-\gamma} - r - \tfrac{(\mu - r)^2}{2 \gamma \sigma^2} \Big], \\
b &= 1.
\end{align*}
$$

Replace 
$$
v(t) = \left( -\frac{1}{a} + \left( v(0)^{-1/\gamma} + \frac{1}{a} \right) e^{-\frac{a}{\gamma} t} \right)^{-\gamma}.
$$

$$
v(t) = \left( -\frac{1}{\rho - \tfrac{1}{1-\gamma} - r - \tfrac{(\mu - r)^2}{2 \gamma \sigma^2}} + \left( v(0)^{-1/\gamma} + \frac{1}{\rho - \tfrac{1}{1-\gamma} - r - \tfrac{(\mu - r)^2}{2 \gamma \sigma^2}} \right) e^{-\frac{\rho - \tfrac{1}{1-\gamma} - r - \tfrac{(\mu - r)^2}{2 \gamma \sigma^2}}{\gamma} t} \right)^{-\gamma}.
$$

---

## Log Utility Solution

### Log Utility Assumptions

**Utility function:**

$$
U(C) = \ln C
$$

**Properties:**

- Constant relative risk aversion: $RRA = 1$
- Elasticity of intertemporal substitution: $EIS = 1$

**Guess for value function:**

$$
V(W,t) = \ln W + u(t)
$$

### Log Utility HJB Solution

**Substitute into HJB:**

$$
\rho (\ln W + u(t)) = \max_{C,\omega} \left\{ \ln C + \frac{\partial V}{\partial t} + V_W [r W + \omega W (\mu - r) - C] + \frac{1}{2} V_{WW} W^2 \omega^2 \sigma^2 \right\}
$$

**Compute derivatives:**

$$
\frac{\partial V}{\partial t} = u'(t),
\frac{\partial V}{\partial W} = \frac{1}{W}, \frac{\partial^2 V}{\partial W^2} = -\frac{1}{W^2}
$$

---

## Continued Log Utility HJB Solution

**Substitute:**

$$
\rho (\ln W + u(t)) = \max_{C,\omega} \left\{ \ln C + u'(t) + \frac{1}{W} [r W + \omega W (\mu - r) - C] - \frac{1}{2} \frac{1}{W^2} W^2 \omega^2 \sigma^2 \right\}
$$

$$
\rho \ln W + \rho u(t) = \max_{C,\omega} \left\{ \ln C + u'(t) + r + \omega (\mu - r) - \frac{C}{W} - \frac{1}{2} \omega^2 \sigma^2 \right\}
$$

**First-order condition for consumption:**

$$
\frac{\partial}{\partial C} [\ln C - \frac{C}{W}] = 0
$$
$$
\frac{1}{C} - \frac{1}{W} = 0
$$
$$
C^* = W
$$

---

## Final Log Utility HJB Solution

**First-order condition for portfolio:**

$$
\frac{\partial}{\partial \omega} [\omega (\mu - r) - \frac{1}{2} \omega^2 \sigma^2] = 0
$$
$$
(\mu - r) - \omega \sigma^2 = 0
$$
$$
\omega^* = \frac{\mu - r}{\sigma^2}
$$

**Substitute back:**

$$
\rho \ln W + \rho u(t) = \ln W + u'(t) + r + \frac{\mu - r}{\sigma^2} (\mu - r) - 1 - \frac{1}{2} \left( \frac{\mu - r}{\sigma^2} \right)^2 \sigma^2
$$

$$
\rho \ln W + \rho u(t) = \ln W + u'(t) + r + \frac{(\mu - r)^2}{\sigma^2} - 1 - \frac{(\mu - r)^2}{2 \sigma^2}
$$

$$
\rho \ln W + \rho u(t) = \ln W + u'(t) + r + \frac{(\mu - r)^2}{2 \sigma^2} - 1
$$

---

## Final Log Utility HJB Solution

**Collect constant terms:**

$$
\rho u(t) = u'(t) + r - 1 + \frac{(\mu - r)^2}{2 \sigma^2}
$$

**ODE for $u(t)$:**

$$
u'(t) = \rho u(t) - r + 1 - \frac{(\mu - r)^2}{2 \sigma^2}
$$

**Solution:**

$$
u(t) = A e^{\rho t} + B
$$

where $A$ and $B$ are constants determined by boundary conditions.

---

## Boundary Conditions and Long-Term Behavior

- How to pin down any constants in the solution?
- Look at behavior at time 0 and as time goes to infinity.
- For example, make the value function bounded as time goes to infinity.
- Value functions at zero normally are set depending on the context of the problem.